get rid of observations in ownP, they just make porting harder

theories/program_logic/ownp.v
@@ -5,69 +5,58 @@ From iris.algebra Require Import auth.
 From iris.proofmode Require Import tactics classes.
 Set Default Proof Using "Type".
 
-Class ownPG' (Λstate Λobservation: Type) (Σ : gFunctors) := OwnPG {
+Class ownPG' (Λstate Λobservation : Type) (Σ : gFunctors) := OwnPG {
   ownP_invG : invG Σ;
-  ownP_state_inG :> inG Σ (authR (optionUR (exclR (leibnizC Λstate))));
-  ownP_obs_inG :> inG Σ (authR (optionUR (exclR (leibnizC (list Λobservation)))));
-  ownP_state_name : gname;
-  ownP_obs_name : gname
+  ownP_inG :> inG Σ (authR (optionUR (exclR (leibnizC Λstate))));
+  ownP_name : gname;
 }.
 Notation ownPG Λ Σ := (ownPG' (state Λ) (observation Λ) Σ).
 
 Instance ownPG_irisG `{ownPG' Λstate Λobservation Σ} : irisG' Λstate Λobservation Σ := {
   iris_invG := ownP_invG;
-  state_interp σ κs := (own ownP_state_name (● (Excl' (σ:leibnizC Λstate))) ∗
-                       own ownP_obs_name (● (Excl' (κs:leibnizC (list Λobservation)))))%I
+  state_interp σ κs := (own ownP_name (● (Excl' (σ:leibnizC Λstate))))%I
 }.
 Global Opaque iris_invG.
 
-Definition ownPΣ (Λstate Λobservation : Type) : gFunctors :=
+Definition ownPΣ (Λstate : Type) : gFunctors :=
   #[invΣ;
-    GFunctor (authR (optionUR (exclR (leibnizC Λstate))));
-    GFunctor (authR (optionUR (exclR (leibnizC (list Λobservation)))))].
+    GFunctor (authR (optionUR (exclR (leibnizC Λstate))))].
 
-Class ownPPreG' (Λstate Λobservation : Type) (Σ : gFunctors) : Set := IrisPreG {
+Class ownPPreG' (Λstate : Type) (Σ : gFunctors) : Set := IrisPreG {
   ownPPre_invG :> invPreG Σ;
-  ownPPre_state_inG :> inG Σ (authR (optionUR (exclR (leibnizC Λstate))));
-  ownPPre_obs_inG :> inG Σ (authR (optionUR (exclR (leibnizC (list Λobservation)))))
+  ownPPre_state_inG :> inG Σ (authR (optionUR (exclR (leibnizC Λstate))))
 }.
-Notation ownPPreG Λ Σ := (ownPPreG' (state Λ) (observation Λ) Σ).
+Notation ownPPreG Λ Σ := (ownPPreG' (state Λ) Σ).
 
-Instance subG_ownPΣ {Λstate Λobservation Σ} : subG (ownPΣ Λstate Λobservation) Σ → ownPPreG' Λstate Λobservation Σ.
+Instance subG_ownPΣ {Λstate Σ} : subG (ownPΣ Λstate) Σ → ownPPreG' Λstate Σ.
 Proof. solve_inG. Qed.
 
 (** Ownership *)
-Definition ownP_state `{ownPG' Λstate Λobservation Σ} (σ : Λstate) : iProp Σ :=
-  own ownP_state_name (◯ (Excl' (σ:leibnizC Λstate))).
+Definition ownP `{ownPG' Λstate Λobservation Σ} (σ : Λstate) : iProp Σ :=
+  own ownP_name (◯ (Excl' (σ:leibnizC Λstate))).
 
-Definition ownP_obs `{ownPG' Λstate Λobservation Σ} (κs: list Λobservation) : iProp Σ :=
-  own ownP_obs_name (◯ (Excl' (κs:leibnizC (list Λobservation)))).
-
-Typeclasses Opaque ownP_state ownP_obs.
-Instance: Params (@ownP_state) 3.
-Instance: Params (@ownP_obs) 3.
+Typeclasses Opaque ownP.
+Instance: Params (@ownP) 3.
 
 (* Adequacy *)
 Theorem ownP_adequacy Σ `{ownPPreG Λ Σ} s e σ φ :
-  (∀ `{ownPG Λ Σ} κs, ownP_state σ ∗ ownP_obs κs ⊢ WP e @ s; ⊤ {{ v, ⌜φ v⌝ }}) →
+  (∀ `{ownPG Λ Σ}, ownP σ ⊢ WP e @ s; ⊤ {{ v, ⌜φ v⌝ }}) →
   adequate s e σ (λ v _, φ v).
 Proof.
   intros Hwp. apply (wp_adequacy Σ _).
   iIntros (? κs).
   iMod (own_alloc (● (Excl' (σ : leibnizC _)) ⋅ ◯ (Excl' σ)))
     as (γσ) "[Hσ Hσf]"; first done.
-  iMod (own_alloc (● (Excl' (κs : leibnizC _)) ⋅ ◯ (Excl' κs)))
-    as (γκs) "[Hκs Hκsf]"; first done.
   iModIntro. iExists (λ σ κs,
-                      own γσ (● (Excl' (σ:leibnizC _))) ∗ own γκs (● (Excl' (κs:leibnizC _))))%I.
-  iFrame "Hσ Hκs".
-  iApply (Hwp (OwnPG _ _ _ _ _ _ γσ γκs)). rewrite /ownP_state /ownP_obs. iFrame.
+                      own γσ (● (Excl' (σ:leibnizC _))))%I.
+  iFrame "Hσ".
+  iApply (Hwp (OwnPG _ _ _ _ _ γσ)). rewrite /ownP. iFrame.
 Qed.
 
 Theorem ownP_invariance Σ `{ownPPreG Λ Σ} s e σ1 t2 σ2 φ :
-  (∀ `{ownPG Λ Σ} κs,
-      ownP_state σ1 ∗ ownP_obs κs ={⊤}=∗ WP e @ s; ⊤ {{ _, True }} ∗
-      |={⊤,∅}=> ∃ σ' κs', ownP_state σ' ∗ ownP_obs κs' ∧ ⌜φ σ'⌝) →
+  (∀ `{ownPG Λ Σ},
+      ownP σ1 ={⊤}=∗ WP e @ s; ⊤ {{ _, True }} ∗
+      |={⊤,∅}=> ∃ σ', ownP σ' ∧ ⌜φ σ'⌝) →
   rtc erased_step ([e], σ1) (t2, σ2) →
   φ σ2.
 Proof.
@@ -75,14 +64,12 @@ Proof.
   iIntros (? κs κs').
   iMod (own_alloc (● (Excl' (σ1 : leibnizC _)) ⋅ ◯ (Excl' σ1)))
     as (γσ) "[Hσ Hσf]"; first done.
-  iMod (own_alloc (● (Excl' (κs ++ κs' : leibnizC _)) ⋅ ◯ (Excl' (κs ++ κs'))))
-    as (γκs) "[Hκs Hκsf]"; first done.
   iExists (λ σ κs',
-           own γσ (● (Excl' (σ:leibnizC _))) ∗ own γκs (● (Excl' (κs':leibnizC _))))%I.
-  iFrame "Hσ Hκs".
-  iMod (Hwp (OwnPG _ _ _ _ _ _ γσ γκs) with "[Hσf Hκsf]") as "[$ H]";
-    first by rewrite /ownP_state /ownP_obs; iFrame.
-  iIntros "!> [Hσ Hκs]". iMod "H" as (σ2' κs'') "[Hσf [Hκsf %]]". rewrite/ownP_state /ownP_obs.
+           own γσ (● (Excl' (σ:leibnizC _))))%I.
+  iFrame "Hσ".
+  iMod (Hwp (OwnPG _ _ _ _ _ γσ) with "[Hσf]") as "[$ H]";
+    first by rewrite /ownP; iFrame.
+  iIntros "!> Hσ". iMod "H" as (σ2') "[Hσf %]". rewrite/ownP.
   iDestruct (own_valid_2 with "Hσ Hσf") as %[Hp _]%auth_valid_discrete_2.
   pose proof (Excl_included _ _ Hp) as Hp'. apply leibniz_equiv in Hp'. inversion Hp'; subst. auto.
 Qed.
@@ -95,65 +82,54 @@ Section lifting.
   Implicit Types e : expr Λ.
   Implicit Types Φ : val Λ → iProp Σ.
 
-  Lemma ownP_eq σ1 σ2 κs1 κs2 : state_interp σ1 κs1 -∗ ownP_state σ2 -∗ ownP_obs κs2 -∗ ⌜σ1 = σ2 ∧ κs1 = κs2⌝.
+  Lemma ownP_eq σ1 σ2 κs : state_interp σ1 κs -∗ ownP σ2 -∗ ⌜σ1 = σ2⌝.
   Proof.
-    iIntros "[Hσ● Hκs●] Hσ◯ Hκs◯". rewrite /ownP_state /ownP_obs.
+    iIntros "Hσ● Hσ◯". rewrite /ownP.
     iDestruct (own_valid_2 with "Hσ● Hσ◯")
       as %[Hps _]%auth_valid_discrete_2.
-    iDestruct (own_valid_2 with "Hκs● Hκs◯")
-      as %[Hpo _]%auth_valid_discrete_2.
     pose proof (leibniz_equiv _ _ (Excl_included _ _ Hps)) as ->.
-    pose proof (leibniz_equiv _ _ (Excl_included _ _ Hpo)) as ->.
     done.
   Qed.
-  Lemma ownP_state_twice σ1 σ2 : ownP_state σ1 ∗ ownP_state σ2 ⊢ False.
-  Proof. rewrite /ownP_state -own_op own_valid. by iIntros (?). Qed.
-  Lemma ownP_obs_twice κs1 κs2 : ownP_obs κs1 ∗ ownP_obs κs2 ⊢ False.
-  Proof. rewrite /ownP_obs -own_op own_valid. by iIntros (?). Qed.
-  Global Instance ownP_state_timeless σ : Timeless (@ownP_state (state Λ) (observation Λ) Σ _ σ).
-  Proof. rewrite /ownP_state; apply _. Qed.
-  Global Instance ownP_obs_timeless κs : Timeless (@ownP_obs (state Λ) (observation Λ) Σ _ κs).
-  Proof. rewrite /ownP_obs; apply _. Qed.
+  Lemma ownP_state_twice σ1 σ2 : ownP σ1 ∗ ownP σ2 ⊢ False.
+  Proof. rewrite /ownP -own_op own_valid. by iIntros (?). Qed.
+  Global Instance ownP_timeless σ : Timeless (@ownP (state Λ) (observation Λ) Σ _ σ).
+  Proof. rewrite /ownP; apply _. Qed.
 
   Lemma ownP_lift_step s E Φ e1 :
-    (|={E,∅}=> ∃ σ1 κs, ⌜if s is NotStuck then reducible e1 σ1 else to_val e1 = None⌝ ∗
-      ▷ ownP_state σ1 ∗ ▷ ownP_obs κs ∗
-      ▷ ∀ κ κs' e2 σ2 efs, ⌜prim_step e1 σ1 κ e2 σ2 efs ∧ κs = κ ++ κs'⌝ -∗
-      ownP_state σ2 ∗ ownP_obs κs'
+    (|={E,∅}=> ∃ σ1, ⌜if s is NotStuck then reducible e1 σ1 else to_val e1 = None⌝ ∗
+      ▷ ownP σ1 ∗
+      ▷ ∀ κ e2 σ2 efs, ⌜prim_step e1 σ1 κ e2 σ2 efs⌝ -∗
+      ownP σ2
             ={∅,E}=∗ WP e2 @ s; E {{ Φ }} ∗ [∗ list] ef ∈ efs, WP ef @ s; ⊤ {{ _, True }})
     ⊢ WP e1 @ s; E {{ Φ }}.
   Proof.
     iIntros "H". destruct (to_val e1) as [v|] eqn:EQe1.
     - apply of_to_val in EQe1 as <-. iApply fupd_wp.
-      iMod "H" as (σ1 κs) "[Hred _]"; iDestruct "Hred" as %Hred.
+      iMod "H" as (σ1) "[Hred _]"; iDestruct "Hred" as %Hred.
       destruct s; last done. apply reducible_not_val in Hred.
       move: Hred; by rewrite to_of_val.
     - iApply wp_lift_step; [done|]; iIntros (σ1 κ κs) "Hσκs".
-      iMod "H" as (σ1' κs' ?) "[>Hσf [>Hκsf H]]".
-      iDestruct (ownP_eq with "Hσκs Hσf Hκsf") as %[<- <-].
+      iMod "H" as (σ1' ?) "[>Hσf H]".
+      iDestruct (ownP_eq with "Hσκs Hσf") as %<-.
       iModIntro; iSplit; [by destruct s|]; iNext; iIntros (e2 σ2 efs Hstep).
-      iDestruct "Hσκs" as "[Hσ Hκs]".
-      rewrite /ownP_state /ownP_obs.
+      iDestruct "Hσκs" as "Hσ". rewrite /ownP.
       iMod (own_update_2 with "Hσ Hσf") as "[Hσ Hσf]".
       { apply auth_update. apply: option_local_update.
          by apply: (exclusive_local_update _ (Excl σ2)). }
-      iMod (own_update_2 with "Hκs Hκsf") as "[Hκs Hκsf]".
-      { apply auth_update. apply: option_local_update.
-        by apply: (exclusive_local_update _ (Excl (κs:leibnizC _))). }
-      iFrame "Hσ Hκs". iApply ("H" with "[]"); eauto with iFrame.
+      iFrame "Hσ". iApply ("H" with "[]"); eauto with iFrame.
   Qed.
 
   Lemma ownP_lift_stuck E Φ e :
-    (|={E,∅}=> ∃ σ κs, ⌜stuck e σ⌝ ∗ ▷ (ownP_state σ ∗ ownP_obs κs))
+    (|={E,∅}=> ∃ σ, ⌜stuck e σ⌝ ∗ ▷ (ownP σ))
     ⊢ WP e @ E ?{{ Φ }}.
   Proof.
     iIntros "H". destruct (to_val e) as [v|] eqn:EQe.
     - apply of_to_val in EQe as <-. iApply fupd_wp.
-      iMod "H" as (σ1 κs) "[H _]". iDestruct "H" as %[Hnv _]. exfalso.
+      iMod "H" as (σ1) "[H _]". iDestruct "H" as %[Hnv _]. exfalso.
       by rewrite to_of_val in Hnv.
     - iApply wp_lift_stuck; [done|]. iIntros (σ1 κs) "Hσ".
-      iMod "H" as (σ1' κs') "(% & >[Hσf Hκsf])".
-      by iDestruct (ownP_eq with "Hσ Hσf Hκsf") as %[-> _].
+      iMod "H" as (σ1') "(% & >Hσf)".
+      by iDestruct (ownP_eq with "Hσ Hσf") as %->.
   Qed.
 
   Lemma ownP_lift_pure_step `{Inhabited (state Λ)} s E Φ e1 :
@@ -173,46 +149,46 @@ Section lifting.
   Qed.
 
   (** Derived lifting lemmas. *)
-  Lemma ownP_lift_atomic_step {s E Φ} e1 σ1 κs :
+  Lemma ownP_lift_atomic_step {s E Φ} e1 σ1 :
     (if s is NotStuck then reducible e1 σ1 else to_val e1 = None) →
-    (▷ (ownP_state σ1 ∗ ownP_obs κs) ∗
-       ▷ ∀ κ κs' e2 σ2 efs, ⌜prim_step e1 σ1 κ e2 σ2 efs ∧ κs = κ ++ κs'⌝ -∗
-         ownP_state σ2 -∗ ownP_obs κs' -∗
+    (▷ (ownP σ1) ∗
+       ▷ ∀ κ e2 σ2 efs, ⌜prim_step e1 σ1 κ e2 σ2 efs⌝ -∗
+         ownP σ2 -∗
       from_option Φ False (to_val e2) ∗ [∗ list] ef ∈ efs, WP ef @ s; ⊤ {{ _, True }})
     ⊢ WP e1 @ s; E {{ Φ }}.
   Proof.
-    iIntros (?) "[[Hσ Hκs] H]"; iApply ownP_lift_step.
+    iIntros (?) "[Hσ H]"; iApply ownP_lift_step.
     iMod (fupd_intro_mask' E ∅) as "Hclose"; first set_solver.
-    iModIntro; iExists σ1, κs; iFrame; iSplit; first by destruct s.
-    iNext; iIntros (κ κs' e2 σ2 efs [??]) "[Hσ Hκs]".
-    iDestruct ("H" $! κ κs' e2 σ2 efs with "[] [Hσ] [Hκs]") as "[HΦ $]"; [by eauto..|].
+    iModIntro; iExists σ1; iFrame; iSplit; first by destruct s.
+    iNext; iIntros (κ e2 σ2 efs ?) "Hσ".
+    iDestruct ("H" $! κ e2 σ2 efs with "[] [Hσ]") as "[HΦ $]"; [by eauto..|].
     destruct (to_val e2) eqn:?; last by iExFalso.
     iMod "Hclose"; iApply wp_value; last done. by apply of_to_val.
   Qed.
 
-  Lemma ownP_lift_atomic_det_step {s E Φ e1} σ1 κ κs v2 σ2 efs :
+  Lemma ownP_lift_atomic_det_step {s E Φ e1} σ1 v2 σ2 efs :
     (if s is NotStuck then reducible e1 σ1 else to_val e1 = None) →
     (∀ κ' e2' σ2' efs', prim_step e1 σ1 κ' e2' σ2' efs' →
-                     κ = κ' ∧ σ2 = σ2' ∧ to_val e2' = Some v2 ∧ efs = efs') →
-    ▷ (ownP_state σ1 ∗ ownP_obs (κ ++ κs)) ∗ ▷ (ownP_state σ2 -∗ ownP_obs κs -∗
+                     σ2 = σ2' ∧ to_val e2' = Some v2 ∧ efs = efs') →
+    ▷ (ownP σ1) ∗ ▷ (ownP σ2 -∗
       Φ v2 ∗ [∗ list] ef ∈ efs, WP ef @ s; ⊤ {{ _, True }})
     ⊢ WP e1 @ s; E {{ Φ }}.
   Proof.
-    iIntros (? Hdet) "[[Hσ1 Hκs] Hσ2]"; iApply ownP_lift_atomic_step; try done.
-    iFrame; iNext; iIntros (κ' κs' e2' σ2' efs' (? & Heq)) "Hσ2' Hκs'".
-    edestruct (Hdet κ') as (->&->&Hval&->); first done. rewrite Hval. apply app_inv_head in Heq as ->.
-    iApply ("Hσ2" with "Hσ2' Hκs'").
+    iIntros (? Hdet) "[Hσ1 Hσ2]"; iApply ownP_lift_atomic_step; try done.
+    iFrame; iNext; iIntros (κ' e2' σ2' efs' ?) "Hσ2'".
+    edestruct (Hdet κ') as (->&Hval&->); first done. rewrite Hval.
+    iApply ("Hσ2" with "Hσ2'").
   Qed.
 
-  Lemma ownP_lift_atomic_det_step_no_fork {s E e1} σ1 κ κs v2 σ2 :
+  Lemma ownP_lift_atomic_det_step_no_fork {s E e1} σ1 v2 σ2 :
     (if s is NotStuck then reducible e1 σ1 else to_val e1 = None) →
     (∀ κ' e2' σ2' efs', prim_step e1 σ1 κ' e2' σ2' efs' →
-      κ = κ' ∧ σ2 = σ2' ∧ to_val e2' = Some v2 ∧ [] = efs') →
-    {{{ ▷ (ownP_state σ1 ∗ ownP_obs (κ ++ κs)) }}} e1 @ s; E {{{ RET v2; ownP_state σ2 ∗ ownP_obs κs}}}.
+      σ2 = σ2' ∧ to_val e2' = Some v2 ∧ [] = efs') →
+    {{{ ▷ (ownP σ1) }}} e1 @ s; E {{{ RET v2; ownP σ2 }}}.
   Proof.
-    intros. rewrite -(ownP_lift_atomic_det_step σ1 κ κs v2 σ2 []); [|done..].
+    intros. rewrite -(ownP_lift_atomic_det_step σ1 v2 σ2 []); [|done..].
     rewrite big_sepL_nil right_id. apply bi.wand_intro_r. iIntros "[Hs Hs']".
-    iSplitL "Hs"; first by iFrame. iModIntro. iIntros "Hσ2 Hκs". iApply "Hs'". iFrame.
+    iSplitL "Hs"; first by iFrame. iModIntro. iIntros "Hσ2". iApply "Hs'". iFrame.
   Qed.
 
   Lemma ownP_lift_pure_det_step `{Inhabited (state Λ)} {s E Φ} e1 e2 efs :
@@ -245,26 +221,26 @@ Section ectx_lifting.
   Hint Resolve head_stuck_stuck.
 
   Lemma ownP_lift_head_step s E Φ e1 :
-    (|={E,∅}=> ∃ σ1 κs, ⌜head_reducible e1 σ1⌝ ∗ ▷ (ownP_state σ1  ∗ ownP_obs κs) ∗
-            ▷ ∀ κ κs' e2 σ2 efs, ⌜head_step e1 σ1 κ e2 σ2 efs ∧ κs = κ ++ κs'⌝ -∗
-            ownP_state σ2 -∗ ownP_obs κs'
+    (|={E,∅}=> ∃ σ1, ⌜head_reducible e1 σ1⌝ ∗ ▷ (ownP σ1) ∗
+            ▷ ∀ κ e2 σ2 efs, ⌜head_step e1 σ1 κ e2 σ2 efs⌝ -∗
+            ownP σ2
             ={∅,E}=∗ WP e2 @ s; E {{ Φ }} ∗ [∗ list] ef ∈ efs, WP ef @ s; ⊤ {{ _, True }})
     ⊢ WP e1 @ s; E {{ Φ }}.
   Proof.
     iIntros "H". iApply ownP_lift_step.
-    iMod "H" as (σ1 κs ?) "[>[Hσ1 Hκs] Hwp]". iModIntro. iExists σ1, κs. iSplit.
+    iMod "H" as (σ1 ?) "[>Hσ1 Hwp]". iModIntro. iExists σ1. iSplit.
     { destruct s; try by eauto using reducible_not_val. }
-    iFrame. iNext. iIntros (κ κs' e2 σ2 efs [? ->]) "[Hσ2 Hκs']".
+    iFrame. iNext. iIntros (κ e2 σ2 efs ?) "Hσ2".
     iApply ("Hwp" with "[] Hσ2"); eauto.
   Qed.
 
   Lemma ownP_lift_head_stuck E Φ e :
     sub_redexes_are_values e →
-    (|={E,∅}=> ∃ σ κs, ⌜head_stuck e σ⌝ ∗ ▷ (ownP_state σ ∗ ownP_obs κs))
+    (|={E,∅}=> ∃ σ, ⌜head_stuck e σ⌝ ∗ ▷ (ownP σ))
     ⊢ WP e @ E ?{{ Φ }}.
   Proof.
-    iIntros (?) "H". iApply ownP_lift_stuck. iMod "H" as (σ κs) "[% >[Hσ Hκs]]".
-    iExists σ, κs. iModIntro. by auto with iFrame.
+    iIntros (?) "H". iApply ownP_lift_stuck. iMod "H" as (σ) "[% >Hσ]".
+    iExists σ. iModIntro. by auto with iFrame.
   Qed.
 
   Lemma ownP_lift_pure_head_step s E Φ e1 :
@@ -279,35 +255,37 @@ Section ectx_lifting.
     iNext. iIntros (?????). iApply "H"; eauto.
   Qed.
 
-  Lemma ownP_lift_atomic_head_step {s E Φ} e1 σ1 κs :
+  Lemma ownP_lift_atomic_head_step {s E Φ} e1 σ1 :
     head_reducible e1 σ1 →
-    ▷ (ownP_state σ1 ∗ ownP_obs κs) ∗ ▷ (∀ κ κs' e2 σ2 efs,
-    ⌜head_step e1 σ1 κ e2 σ2 efs ∧ κs = κ ++ κs'⌝ -∗ ownP_state σ2 -∗ ownP_obs κs' -∗
+    ▷ (ownP σ1) ∗ ▷ (∀ κ e2 σ2 efs,
+    ⌜head_step e1 σ1 κ e2 σ2 efs⌝ -∗ ownP σ2 -∗
       from_option Φ False (to_val e2) ∗ [∗ list] ef ∈ efs, WP ef @ s; ⊤ {{ _, True }})
     ⊢ WP e1 @ s; E {{ Φ }}.
   Proof.
     iIntros (?) "[Hst H]". iApply ownP_lift_atomic_step; eauto.
     { by destruct s; eauto using reducible_not_val. }
     iSplitL "Hst"; first done.
-    iNext. iIntros (????? [? ->]) "Hσ ?". iApply ("H" with "[] Hσ"); eauto.
+    iNext. iIntros (???? ?) "Hσ". iApply ("H" with "[] Hσ"); eauto.
   Qed.
 
-  Lemma ownP_lift_atomic_det_head_step {s E Φ e1} σ1 κ κs v2 σ2 efs :
+  Lemma ownP_lift_atomic_det_head_step {s E Φ e1} σ1 v2 σ2 efs :
     head_reducible e1 σ1 →
     (∀ κ' e2' σ2' efs', head_step e1 σ1 κ' e2' σ2' efs' →
-      κ = κ' ∧ σ2 = σ2' ∧ to_val e2' = Some v2 ∧ efs = efs') →
-    ▷ (ownP_state σ1 ∗ ownP_obs (κ ++ κs)) ∗ ▷ (ownP_state σ2 -∗ ownP_obs κs -∗
-                                                    Φ v2 ∗ [∗ list] ef ∈ efs, WP ef @ s; ⊤ {{ _, True }})
+      σ2 = σ2' ∧ to_val e2' = Some v2 ∧ efs = efs') →
+    ▷ (ownP σ1) ∗ ▷ (ownP σ2 -∗
+                      Φ v2 ∗ [∗ list] ef ∈ efs, WP ef @ s; ⊤ {{ _, True }})
     ⊢ WP e1 @ s; E {{ Φ }}.
   Proof.
-    intros Hr Hs. destruct s; apply ownP_lift_atomic_det_step; eauto using reducible_not_val.
+    intros Hr Hs.
+    destruct s; apply ownP_lift_atomic_det_step; eauto using reducible_not_val;
+    intros; eapply Hs; eauto 10.
   Qed.
 
-  Lemma ownP_lift_atomic_det_head_step_no_fork {s E e1} σ1 κ κs v2 σ2 :
+  Lemma ownP_lift_atomic_det_head_step_no_fork {s E e1} σ1 κ v2 σ2 :
     head_reducible e1 σ1 →
     (∀ κ' e2' σ2' efs', head_step e1 σ1 κ' e2' σ2' efs' →
       κ = κ' ∧ σ2 = σ2' ∧ to_val e2' = Some v2 ∧ [] = efs') →
-    {{{ ▷ (ownP_state σ1 ∗ ownP_obs (κ ++ κs)) }}} e1 @ s; E {{{ RET v2; ownP_state σ2 ∗ ownP_obs κs }}}.
+    {{{ ▷ (ownP σ1) }}} e1 @ s; E {{{ RET v2; ownP σ2 }}}.
   Proof.
     intros ???; apply ownP_lift_atomic_det_step_no_fork; last naive_solver.
     by destruct s; eauto using reducible_not_val.
